Bdd/Prime.lean
@@ -1,0 +1,376 @@
+import Bdd.Basic
+
+namespace Prime
+
+def prime_node (p : Nat): Node n m → Node (n + p) m
+  | ⟨var, low, high⟩ => ⟨⟨var.1 + p, (add_lt_add_iff_right p).mpr (Fin.is_lt var)⟩, low, high⟩
+
+def prime_heap (p : Nat): Vector (Node n m) m → Vector (Node (n + p) m) m := Vector.map (prime_node p)
+
+def prime (p : Nat) : Bdd n m → Bdd (n + p) m
+  | ⟨heap, root⟩ => ⟨prime_heap p heap, root⟩
+
+lemma prime_edge_iff {B : Bdd n m} {x y : Pointer m} : Edge B.heap x y ↔ Edge (prime p B).heap x y := by
+  constructor
+  · intro e
+    cases e with
+    | low  _ => left;  simpa [prime, prime_heap, prime_node]
+    | high _ => right; simpa [prime, prime_heap, prime_node]
+  · intro e
+    cases e with
+    | low  _ => left;  simp_all [prime, prime_heap, prime_node]; assumption
+    | high _ => right; simp_all [prime, prime_heap, prime_node]; assumption
+
+lemma prime_reachable_iff {B : Bdd n m} : Pointer.Reachable B.heap B.root x ↔ Pointer.Reachable (prime p B).heap (prime p B).root x := by
+  constructor
+  · intro r
+    induction r with
+    | refl => left
+    | tail _ e ih =>
+      right
+      · exact ih
+      · exact (prime_edge_iff.mp e)
+  · intro r
+    induction r with
+    | refl => left
+    | tail _ e ih =>
+      right
+      · exact ih
+      · exact (prime_edge_iff.mpr e)
+
+lemma prime_mayPrecede_iff {B : Bdd n m} {x y : Pointer m}: Pointer.MayPrecede B.heap x y ↔ Pointer.MayPrecede (prime p B).heap x y := by
+  constructor
+  · intro h
+    cases x with
+    | terminal _ => absurd h; exact Pointer.not_terminal_MayPrecede
+    | node _ =>
+      cases y with
+      | terminal _ => apply Pointer.MayPrecede_node_terminal
+      | node _ =>
+        simp only [Pointer.MayPrecede, prime, prime_heap, Pointer.toVar] at h
+        simp only [Nat.succ_eq_add_one, Fin.getElem_fin, Fin.coe_eq_castSucc, Fin.castSucc_lt_castSucc_iff] at h
+        simp only [Pointer.MayPrecede, prime, prime_heap, Pointer.toVar]
+        simp only [Nat.succ_eq_add_one, Fin.getElem_fin, Vector.getElem_map, Fin.coe_eq_castSucc, Fin.castSucc_lt_castSucc_iff]
+        simp only [prime_node]
+        simp only [Fin.eta, Fin.mk_lt_mk, add_lt_add_iff_right, Fin.val_fin_lt]
+        exact h
+  · intro h
+    cases x with
+    | terminal _ => absurd h; exact Pointer.not_terminal_MayPrecede
+    | node _ =>
+      cases y with
+      | terminal _ => apply Pointer.MayPrecede_node_terminal
+      | node _ =>
+        simp only [Pointer.MayPrecede, prime, prime_heap, Pointer.toVar]
+        simp only [Nat.succ_eq_add_one, Fin.getElem_fin, Fin.coe_eq_castSucc, Fin.castSucc_lt_castSucc_iff]
+        simp only [Pointer.MayPrecede, prime, prime_heap, Pointer.toVar] at h
+        simp only [Nat.succ_eq_add_one, Fin.getElem_fin, Vector.getElem_map, Fin.coe_eq_castSucc, Fin.castSucc_lt_castSucc_iff] at h
+        simp only [prime_node] at h
+        simp only [Fin.eta, Fin.mk_lt_mk, add_lt_add_iff_right, Fin.val_fin_lt] at h
+        exact h
+
+lemma prime_relevantMayPrecede {B : Bdd n m} {x y : Pointer m} {hx : Pointer.Reachable (prime p B).heap (prime p B).root x} {hy : Pointer.Reachable (prime p B).heap (prime p B).root y} :
+    B.RelevantMayPrecede ⟨x, prime_reachable_iff.mpr hx⟩ ⟨y, prime_reachable_iff.mpr hy⟩ → (prime p B).RelevantMayPrecede ⟨x, hx⟩ ⟨y, hy⟩ := prime_mayPrecede_iff.mp
+
+lemma prime_relevantEdge {B : Bdd n m} {x y : Pointer m} {hx : Pointer.Reachable (prime p B).heap (prime p B).root x} {hy : Pointer.Reachable (prime p B).heap (prime p B).root y} :
+    (prime p B).RelevantEdge ⟨x, hx⟩ ⟨y, hy⟩ → B.RelevantEdge ⟨x, prime_reachable_iff.mpr hx⟩ ⟨y, prime_reachable_iff.mpr hy⟩ := by
+  intro h
+  simp_all only [Bdd.RelevantEdge, prime, prime_heap]
+  cases h with
+  | low _ =>
+    left
+    simp_all [prime_node]
+    assumption
+  | high _ =>
+    right
+    simp_all [prime_node]
+    assumption
+
+lemma prime_preserves_ordered : Bdd.Ordered B → Bdd.Ordered (prime p B) := by
+  intro ho
+  rintro _ _ hxy
+  apply prime_relevantMayPrecede
+  apply ho
+  exact prime_relevantEdge hxy
+
+def oprime p : OBdd n m → OBdd (n + p) m
+  | O => ⟨prime p O.1, prime_preserves_ordered O.2⟩
+
+lemma oprime_low {n m j p} {O : OBdd n m} {h : O.1.root = .node j} : (OBdd.low (oprime p O) h) = oprime p (O.low h) := by
+  rcases O with ⟨B, o⟩
+  simp only [OBdd.low]
+  congr
+  simp only [oprime, prime, prime_heap, Bdd.low_heap_eq_heap]
+  simp only at h
+  simp_rw [h]
+  simp only [Bdd.low]
+  congr 1
+  simp_all only [Fin.getElem_fin, Vector.getElem_map]
+  rfl
+
+lemma oprime_high {n m j p} {O : OBdd n m} {h : O.1.root = .node j} : (OBdd.high (oprime p O) h) = oprime p (O.high h) := by
+  rcases O with ⟨B, o⟩
+  simp only [OBdd.high]
+  congr
+  simp only [oprime, prime, prime_heap, Bdd.high_heap_eq_heap]
+  simp only at h
+  simp_rw [h]
+  simp only [Bdd.high]
+  congr 1
+  simp_all only [Fin.getElem_fin, Vector.getElem_map]
+  rfl
+
+lemma bprime_low {n m j p} {B : Bdd n m} {o : Bdd.Ordered B} {h : B.root = .node j} : (OBdd.low ⟨prime p B, prime_preserves_ordered o⟩ h) = ⟨prime p (OBdd.low ⟨B, o⟩ h).1, prime_preserves_ordered (OBdd.low ⟨B, o⟩ h).2⟩ := by
+  simp only [OBdd.low]
+  congr
+  simp only [prime, prime_heap, Bdd.low_heap_eq_heap]
+  simp_rw [h]
+  simp only [Bdd.low]
+  congr 1
+  simp_all only [Fin.getElem_fin, Vector.getElem_map]
+  rfl
+
+lemma bprime_high {n m j p} {B : Bdd n m} {o : Bdd.Ordered B} {h : B.root = .node j} : (OBdd.high ⟨prime p B, prime_preserves_ordered o⟩ h) = ⟨prime p (OBdd.high ⟨B, o⟩ h).1, prime_preserves_ordered (OBdd.high ⟨B, o⟩ h).2⟩ := by
+  simp only [OBdd.high]
+  congr
+  simp only [prime, prime_heap, Bdd.high_heap_eq_heap]
+  simp_rw [h]
+  simp only [Bdd.high]
+  congr 1
+  simp_all only [Fin.getElem_fin, Vector.getElem_map]
+  rfl
+
+lemma prime_low {n m j p} {O : OBdd n m} {h : O.1.root = .node j} : (OBdd.low ⟨prime p O.1, prime_preserves_ordered O.2⟩ h) = ⟨prime p (O.low h).1, prime_preserves_ordered (O.low h).2⟩ := by
+  simp only [OBdd.low]
+  congr
+  simp only [prime, prime_heap, Bdd.low_heap_eq_heap]
+  simp_rw [h]
+  simp only [Bdd.low]
+  congr 1
+  simp_all only [Fin.getElem_fin, Vector.getElem_map]
+  rfl
+
+lemma prime_high {n m j p} {O : OBdd n m} {h : O.1.root = .node j} : (OBdd.high ⟨prime p O.1, prime_preserves_ordered O.2⟩ h) = ⟨prime p (O.high h).1, prime_preserves_ordered (O.high h).2⟩ := by
+  simp only [OBdd.high]
+  congr
+  simp only [prime, prime_heap, Bdd.high_heap_eq_heap]
+  simp_rw [h]
+  simp only [Bdd.high]
+  congr 1
+  simp_all only [Fin.getElem_fin, Vector.getElem_map]
+  rfl
+
+theorem oprime_evaluate (O : OBdd n m) : OBdd.evaluate (oprime p O) I = O.evaluate (Vector.cast (show n + p - p = n from Eq.symm (Nat.eq_sub_of_add_eq rfl)) (I.drop p)) := by
+  simp only [oprime]
+  cases O_root_def : O.1.root with
+  | terminal _ =>
+    simp only [prime]
+    rw [OBdd.evaluate_terminal' O_root_def]
+    simp_rw [O_root_def]
+    rw [OBdd.evaluate_terminal]
+    simp
+  | node j =>
+    rw [OBdd.evaluate_node'' O_root_def]
+    have that : (⟨(prime p O.1), prime_preserves_ordered O.2⟩ : OBdd _ _).1.root = Pointer.node j := O_root_def
+    rw [OBdd.evaluate_node'' that]
+    simp only
+    congr 1
+    · simp only [eq_iff_iff, Bool.coe_iff_coe]
+      simp only [prime, prime_heap, Fin.getElem_fin, Vector.getElem_map, prime_node]
+      simp only [Fin.eta]
+      rw [Vector.getElem_cast]
+      symm
+      simp_rw [add_comm]
+      apply Vector.getElem_drop
+    · have := oprime_evaluate (O.high O_root_def) (I := I)
+      rw [← this]
+      rw [← oprime_high]
+      rfl
+    · have := oprime_evaluate (O.low O_root_def) (I := I)
+      rw [← this]
+      rw [← oprime_low]
+      rfl
+termination_by O
+
+theorem prime_evaluate (O : OBdd n m) : OBdd.evaluate ⟨prime p O.1, prime_preserves_ordered O.2⟩ I = O.evaluate (Vector.cast (show n + p - p = n from Eq.symm (Nat.eq_sub_of_add_eq rfl)) (I.drop p)) := by
+  cases O_root_def : O.1.root with
+  | terminal _ =>
+    simp only [prime]
+    rw [OBdd.evaluate_terminal' O_root_def]
+    simp_rw [O_root_def]
+    rw [OBdd.evaluate_terminal]
+    simp
+  | node j =>
+    rw [OBdd.evaluate_node'' O_root_def]
+    have that : (⟨(prime p O.1), prime_preserves_ordered O.2⟩ : OBdd _ _).1.root = Pointer.node j := O_root_def
+    rw [OBdd.evaluate_node'' that]
+    simp only
+    congr 1
+    · simp only [eq_iff_iff, Bool.coe_iff_coe]
+      simp only [prime, prime_heap, Fin.getElem_fin, Vector.getElem_map, prime_node]
+      simp only [Fin.eta]
+      rw [Vector.getElem_cast]
+      symm
+      simp_rw [add_comm]
+      apply Vector.getElem_drop
+    · have := prime_evaluate (O.high O_root_def) (I := I)
+      rw [← this]
+      rw [← prime_high]
+    · have := prime_evaluate (O.low O_root_def) (I := I)
+      rw [← this]
+      rw [← prime_low]
+termination_by O
+
+lemma prime_preserves_noRedundancy {B : Bdd n m} : B.NoRedundancy → (prime p B).NoRedundancy := by
+  rintro hnr ⟨p, hp⟩ contra
+  simp only at contra
+  cases p_def : p with
+  | terminal _ =>
+    cases contra with
+    | red _ => contradiction
+  | node j =>
+    rw [p_def] at contra
+    cases contra with
+    | red red =>
+      simp only [prime, prime_heap, Fin.getElem_fin, prime_node] at red
+      apply hnr ⟨p, prime_reachable_iff.mpr hp⟩
+      simp_rw [p_def]
+      constructor
+      simp_all only [Vector.getElem_map, Fin.getElem_fin]
+      simp only [prime, prime_heap, Fin.getElem_fin, prime_node] at red
+      exact red
+
+def tprime p : DecisionTree n → DecisionTree (n + p)
+  | .leaf b => .leaf b
+  | .branch i l h => .branch ⟨i.1 + p, by omega⟩ (tprime p l) (tprime p h)
+
+lemma tprime_injective : Function.Injective (tprime (n := n) p) := by
+  intro x y hxy
+  cases x with
+  | leaf _ =>
+    cases y with
+    | leaf _ => simp only [tprime] at hxy; simp_all
+    | branch _ _ _ => contradiction
+  | branch _ _ _ =>
+    cases y with
+    | leaf _ => contradiction
+    | branch _ _ _ =>
+      simp only [tprime] at hxy
+      injection hxy with a b c
+      rw [tprime_injective b, tprime_injective c]
+      aesop
+
+lemma prime_toTree_tprime' {O : OBdd n m} :
+    OBdd.toTree ⟨prime p O.1, prime_preserves_ordered O.2⟩ = tprime p (OBdd.toTree O) := by
+  cases O_root_def : O.1.root with
+  | terminal _ =>
+    simp only [prime]
+    rw [OBdd.toTree_terminal' O_root_def]
+    simp_rw [O_root_def]
+    rw [OBdd.toTree_terminal]
+    simp [tprime]
+  | node _ =>
+    -- simp only [prime]
+    rw [OBdd.toTree_node O_root_def]
+    rw [OBdd.toTree_node (by trans O.1.root; rfl; exact O_root_def)]
+    simp only [Fin.getElem_fin]
+    congr 1
+    · simp only [prime, prime_heap, Vector.getElem_map, prime_node, Fin.eta, Bdd.Ordered.eq_1, Fin.mk.injEq, Nat.add_right_cancel_iff]
+      rfl
+    · have := prime_toTree_tprime' (O := (O.low O_root_def)) (p := p)
+      rw [← prime_low] at this
+      exact this
+    · have := prime_toTree_tprime' (O := (O.high O_root_def)) (p := p)
+      rw [← prime_high] at this
+      exact this
+termination_by O
+
+lemma prime_toTree_tprime {B : Bdd n m} {o : B.Ordered} :
+    OBdd.toTree ⟨prime p B, prime_preserves_ordered o⟩ = tprime p (OBdd.toTree ⟨B, o⟩) := by
+  let O : OBdd n m := ⟨B, o⟩
+  have : B = O.1 := rfl
+  simp_rw [this]
+  exact prime_toTree_tprime'
+
+lemma oprime_preserves_similarRP {O : OBdd n m} {p q : Pointer m} {hp : Pointer.Reachable (oprime x O).1.heap (oprime x O).1.root p} {hq : Pointer.Reachable (oprime x O).1.heap (oprime x O).1.root q} :
+    (oprime x O).SimilarRP ⟨p, hp⟩ ⟨q, hq⟩ → O.SimilarRP ⟨p, prime_reachable_iff.mpr hp⟩ ⟨q, prime_reachable_iff.mpr hq⟩ := by
+  intro sim
+  simp only [OBdd.SimilarRP, OBdd.Similar, OBdd.HSimilar] at sim
+  simp only [OBdd.SimilarRP, OBdd.Similar, OBdd.HSimilar]
+  cases p with
+  | terminal _ =>
+    cases q with
+    | terminal _ => simp_all
+    | node _ =>
+      simp only [OBdd.toTree_terminal] at sim
+      rw [OBdd.toTree_node rfl] at sim
+      contradiction
+  | node j =>
+    cases q with
+    | terminal _ =>
+      simp only [OBdd.toTree_terminal] at sim
+      rw [OBdd.toTree_node rfl] at sim
+      contradiction
+    | node i =>
+      conv at sim =>
+        lhs
+        rw [OBdd.toTree_node rfl]
+      conv at sim =>
+        rhs
+        rw [OBdd.toTree_node rfl]
+      injection sim with ha hb hc
+      simp only [Fin.getElem_fin] at ha
+      simp only [oprime, prime, prime_heap, Vector.getElem_map, prime_node, Fin.eta, Fin.mk.injEq, Nat.add_right_cancel_iff] at ha
+      conv =>
+        lhs
+        rw [OBdd.toTree_node rfl]
+      conv =>
+        rhs
+        rw [OBdd.toTree_node rfl]
+      congr 1
+      · simp only
+        exact Fin.eq_of_val_eq ha
+      · simp only [oprime] at hb
+        simp only [prime] at hb
+        simp_rw [← prime.eq_1] at hb
+        conv at hb =>
+          lhs
+          rw [bprime_low (h := rfl) (o := Bdd.ordered_of_reachable (prime_reachable_iff.mpr hp))]
+        conv at hb =>
+          rhs
+          rw [bprime_low (h := rfl) (o := Bdd.ordered_of_reachable (prime_reachable_iff.mpr hq))]
+        simp only [OBdd.low] at hb
+        simp only [OBdd.low]
+        conv at hb =>
+          lhs
+          rw [prime_toTree_tprime (o := (by apply Bdd.low_ordered; exact Bdd.ordered_of_reachable (prime_reachable_iff.mpr hp)))]
+        conv at hb =>
+          rhs
+          rw [prime_toTree_tprime (o := (by apply Bdd.low_ordered; exact Bdd.ordered_of_reachable (prime_reachable_iff.mpr hq)))]
+        rw [tprime_injective hb]
+      · simp only [oprime] at hc
+        simp only [prime] at hc
+        simp_rw [← prime.eq_1] at hc
+        conv at hc =>
+          lhs
+          rw [bprime_high (h := rfl) (o := Bdd.ordered_of_reachable (prime_reachable_iff.mpr hp))]
+        conv at hc =>
+          rhs
+          rw [bprime_high (h := rfl) (o := Bdd.ordered_of_reachable (prime_reachable_iff.mpr hq))]
+        simp only [OBdd.high] at hc
+        simp only [OBdd.high]
+        conv at hc =>
+          lhs
+          rw [prime_toTree_tprime (o := (by apply Bdd.high_ordered; exact Bdd.ordered_of_reachable (prime_reachable_iff.mpr hp)))]
+        conv at hc =>
+          rhs
+          rw [prime_toTree_tprime (o := (by apply Bdd.high_ordered; exact Bdd.ordered_of_reachable (prime_reachable_iff.mpr hq)))]
+        rw [tprime_injective hc]
+
+lemma oprime_reduced {O : OBdd n m} : O.Reduced → (oprime p O).Reduced := by
+  rintro ⟨r1, r2⟩
+  constructor
+  · exact prime_preserves_noRedundancy r1
+  · rintro _ _ sim; exact r2 (oprime_preserves_similarRP sim)
+
+end Prime
